\input{Imports.tex}
\begin{document}
\section{Solving the simple discounted problem}
We are going to solve problem with the following Bellman equations:
$$
J(l,1)=\min\{
c+e^{-\alpha dt} J(0,1),
e^{-\alpha dt} \mathbb{E}[J(l+dt,I(t_{k+1}))]
\}.
$$
$$
J(l,0)=c + a + e^{-\alpha h} J(0,1).
$$
Where $I(t_{k+1})$ is a random variable and it is $0$ if $l<Q_{n(t_k)}<l+dt$ and $1$ else. Let the $Q_i$'s have cdf $F(.)$, pdf $f(.)$, hazard rate $h(.)$ and cumulative hazard rate $H(.)$. Then
$$
\mathbb{P}(l<Q_{n(t_k)}<l+dt|l<Q_{n(t_k)})=\mathbb{P}(l<Q_0<l+dt|l<Q_0)
$$
$$
=\frac{F(l+dt)-F(l)}{1-F(l)}=\frac{dt\,f(l)+o(dt^2)}{1-F(l)}=dt\,h(l)+o(dt^2).
$$
So that $I(t_{k+1})=0$ with probability $dth(l)+o(h^2)$ and $1$ with probability $1-dt\,h(l)+o(dt^2)$. Resulting in
$$
J(l,1)=\min\{
c+e^{-\alpha dt} J(0,1), 
e^{-\alpha dt} [dt\,h(l)J(l+dt,0) + (1-dt\,h(l))J(l+dt,1) +o(dt^2)]
\}.
$$
When we assume that $J(l+dt,1)<c+e^{-\alpha dt} J(0,1)$, we can write
$$
J(l,1)=
(1-\alpha dt +o(dt^2)) [dt\,h(l)J(l+dt,0) + (1-dt\,h(l))J(l+dt,1) +o(dt^2)]
$$
$$
=dt\,h(l)J(l+dt,0) + (1-dt\,h(l))J(l+dt,1) - \alpha dt J(l+dt,1) +o(dt^2)
.
$$
Or equivalently
$$
J(l,1)-J(l+dt,1)=
dt[h(l)J(l+h,0) - (\alpha +h(l))J(l+dt,1)] +o(dt^2)
.
$$
Dividing by $-dt$ results in
$$
\frac{J(l+dt,1)-J(l,1)}{dt}=
-h(l)J(l+dt,0) + (\alpha +h(l))J(l+dt,1) +o(dt)
.
$$
Since we know that $J(l+dt,0)=c + a + e^{-\alpha dt} J(0,1)=c+a+(1+o(dt))J(0,1)$, we can write
$$
\frac{J(l+dt,1)-J(l,1)}{dt}=
-h(l)(c+a+J(0,1)) + (\alpha +h(l))J(l+dt,1) +o(dt)
.
$$
If we let $dt$ approach $0$, this results in
$$
\frac{d}{dl}J(l,1)=
-h(l)(c+a+J(0,1)) + (\alpha +h(l))J(l,1)
.
$$
Which seems counterintuitive since for small $\alpha$, $J(l,1)$ would be decreasing as $J(l,1)<c+e^{-\alpha dt} J(0,1)<c+a+J(0,1)$.
We will try to solve this O.D.E. anyway.
We use the method of the integrating factor.
Our integrating factor will be
$$
e^{\int\limits_0^l (-\alpha - h(x))dx}=e^{-\alpha l -H(l)}.
$$
So that we get
$$
J(l,1)=e^{\alpha l +H(l)} [C + \int\limits_0^l e^{-\alpha x -H(x)}(-h(x)(c+a+J(0,1)))dx]
$$
$$
=\frac{e^{\alpha l}}{1-F(l)} [C - (c+a+J(0,1))\int\limits_0^l e^{-\alpha x}f(x)dx].
$$
Using the identities $e^{H(l)}=(e^{-H(l)})^{-1}=\frac{1}{1-F(l)}$ and $h(l)e^{-H(l)}=f(l)$.
The $C$ is an integrating constant and since $J(l)=J(0,1)$ should hold, we find $C=J(0,1)$.
We can rewrite the expression to
$$
J(l,1)=\frac{e^{\alpha l}}{1-F(l)} [J(0,1)  - (c+a+J(0,1))\mathbb{P}(L<l)\mathbb{E}[e^{-\alpha L}|L<l]].
$$
Concluding
$$
J(l,1)=\min\{
c+J(0,1),
\frac{ e^{\alpha l}}{1-F(l)} [J(0,1) - (c+a+J(0,1))\mathbb{P}(L<l)\mathbb{E}[e^{-\alpha L}|L<l]]
\}
$$
and preventive maintenance is chosen if and only if $J(l,1)=c+J(0,1)$.
However, the value of $J(0,1)$ depends on the policy that is chosen and it seems difficult to solve $J(l,1)=c+J(0,1)$ analytically for $l$.
\end{document}